\section*{Question 3}
Suppose on the contrary that $ a + b $, $ b + c $ and $ c + a $ are linearly dependent, then there exists $ p $, $ q $ and $ r $ not all zero so that $ p(a+b) + q(b + c) + r(c + a) = 0 $, which implies $ (p + r)a + (p + q)b + (q + r)c = 0 $. Because $ a $, $ b $ and $ c $ are linearly independent, $ (p+r) = (p+q) = (q+r) = 0 $. 

Taking a sum of these equations give $ 2(p + q + r) = 0 $, which implies $ p + q + r = 0 $.

Subtracting the equations from $ p + q + r = 0 $ shows $ p = q = r = 0 $.

But we started with $ p $, $ q $ and $ r $ not all zero, so this contradiction shows $ a + b $, $ b + c $ and $ c + a $ are linearly independent.