\section*{Question 12}
\subsection*{Part a}
\subsubsection*{Part i}
\begin{eqnarray*}
  \Delta \ge 0 \\
  b^2 - 4ac \ge 0 \\
  (-2p)^2 - 4(1)(q) \ge 0 \\
  4p^2 - 4q \ge 0 \\
  p^2 \ge q
\end{eqnarray*}
\subsubsection*{Part ii}
\begin{eqnarray*}
    -3b &=& -(\alpha + \beta + \gamma) \\
        &=& -((2p) + \gamma) \\
      b &=& \frac{2p + \gamma}{3}
\end{eqnarray*}

\begin{eqnarray*}
    3c &=& \alpha\beta + \alpha\gamma + \beta\gamma \\
       &=& q + (\alpha + \beta)\gamma \\
       &=& q + 2p\gamma \\
     c &=& \frac{q + 2p\gamma}{3}
\end{eqnarray*}

\begin{eqnarray*}
    -d &=& -\alpha\beta\gamma \\
     d &=& q\gamma
\end{eqnarray*}

To prove the inequalities, we start with these few simple results:

\begin{eqnarray*}
  (p - \gamma)^2 &\ge& 0 \\
  p^2 - 2p\gamma + \gamma^2 &\ge& 0 \\
  p^2 + 4p\gamma + \gamma^2 &\ge& 6p\gamma \\
\end{eqnarray*}

\begin{eqnarray*}
  p^2 &\ge& q \\
  3p^2 &\ge& 3q
\end{eqnarray*}

Combining them, we can get:

\begin{eqnarray*}
  3p^2 + p^2 + 4p\gamma + \gamma^2 &\ge& 3q + 6p\gamma \\
  4p^2 + 4p\gamma + \gamma^2 &\ge& 3q + 6p\gamma \\
  \frac{4p^2 + 4p\gamma + \gamma^2}{9} &\ge& \frac{3q + 6p\gamma}{9} \\
  \frac{4p^2 + 4p\gamma + \gamma^2}{9} &\ge& \frac{q + 2p\gamma}{3} \\
  \left(\frac{2p + \gamma}{3}\right)^2 &\ge& \frac{q + 2p\gamma}{3} \\
  b^2 \ge c
\end{eqnarray*}

$ 2p = \alpha + \beta > 0 $, $ q = \alpha \beta > 0 $, $ \gamma > 0 $, so $ c > 0 $. \\

For the other inequality, we can use a similar trick:

\begin{eqnarray*}
  (q - p\gamma)^2 &\ge& 0 \\
  q^2 - 2pq\gamma + p^2\gamma^2 &\ge& 0 \\
  q^2 + 4pq\gamma + p^2\gamma^2 &\ge& 6pq\gamma 
\end{eqnarray*}

\begin{eqnarray*}
  p^2 &\ge& q \\
  3p^2\gamma^2 &\ge& 3q\gamma^2
\end{eqnarray*}

Combining:

\begin{eqnarray*}
  q^2 + 4pq\gamma + p^2\gamma^2 + 3p^2\gamma^2 &\ge& 6pq\gamma + 3q\gamma^2 \\
  q^2 + 4pq\gamma + 4p^2\gamma^2 &\ge& 6pq\gamma + 3q\gamma^2 \\
  q^2 + 4pq\gamma + 4p^2\gamma^2 &\ge& (6p + 3\gamma)q\gamma \\
  \frac{q^2 + 4pq\gamma + 4p^2\gamma^2}{9} &\ge& \left(\frac{6p + 3\gamma}{9}\right)q\gamma \\
  \frac{q^2 + 4pq\gamma + 4p^2\gamma^2}{9} &\ge& \left(\frac{2p + \gamma}{3}\right) q\gamma \\
  c^2 & \ge & bd 
\end{eqnarray*}

Last, but not least, 

\begin{eqnarray*}
  b^2 &\ge& c \\
  b &\ge& \sqrt{c} \\
  bdc &\ge& c\sqrt{c}d \\
  (c^2)c &\ge& c\sqrt{c}d \\
  (\sqrt{c})^3 &\ge& d \\
  \sqrt{c} &\ge& \sqrt[3]{d}
\end{eqnarray*}

\subsection*{Part 2}
Note that $ B = \frac{\pi - A - C}{2} = \frac{\pi}{2} - \frac{(A+C)}{2} $, so $ \tan\left(\frac{B}{2}\right) = \frac{1}{\tan(\frac{A}{2}+\frac{C}{2})} $

Now we consider the latter:
\begin{eqnarray*}
  \tan\left(\frac{A}{2}+\frac{C}{2}\right) &=& \frac{\tan\left(\frac{A}{2}\right) + \tan\left(\frac{C}{2}\right)}{1 - \tan\left(\frac{A}{2}\right)\tan\left(\frac{C}{2}\right)} \\
  \tan\left(\frac{B}{2}\right) &=& \frac{1 - \tan\left(\frac{A}{2}\right)\tan\left(\frac{C}{2}\right)}{\tan\left(\frac{A}{2}\right) + \tan\left(\frac{C}{2}\right)} \\
  \tan\left(\frac{B}{2}\right)\left(\tan\left(\frac{A}{2}\right) + \tan\left(\frac{C}{2}\right)\right) &=& 1 - \tan\left(\frac{A}{2}\right)\tan\left(\frac{C}{2}\right) \\
  \tan\left(\frac{A}{2}\right)\tan\left(\frac{B}{2}\right) + \tan\left(\frac{B}{2}\right)\tan\left(\frac{C}{2}\right) + \tan\left(\frac{C}{2}\right)\tan\left(\frac{A}{2}\right) &=& 1
\end{eqnarray*}

Using part (a) and consider $ (\alpha, \beta, \gamma) = (\tan\left(\frac{A}{2}\right), \tan\left(\frac{B}{2}\right), \tan\left(\frac{C}{2}\right)) $, these are obviously positive numbers.

First, let's figure out the values for $ b $, $ c $ and $ d $.
\begin{eqnarray*}
  b &=& \frac{\alpha + \beta + \gamma}{3} \\
  c &=& \frac{1}{3}(\alpha\beta + \beta\gamma + \gamma\alpha) \\
    &=& \frac{1}{3} \\
  d &=& \alpha \beta \gamma
\end{eqnarray*}

Then we can use the results:
\begin{eqnarray*}
  b &\ge& \sqrt{c} \\
  \frac{\alpha + \beta + \gamma}{3} &\ge& \sqrt{\frac{1}{3}} \\
  \alpha + \beta + \gamma &\ge& \sqrt{3}
\end{eqnarray*}

\begin{eqnarray*}
  \sqrt[3]{d} &\;e& \sqrt{c} \\
  d &\le& c^{3}{2} \\
  \alpha \beta \gamma &\le& \left(\frac{1}{3}\right)^{\frac{3}{2}} \\
                      &=& \frac{\sqrt{3}}{9}
\end{eqnarray*}