\section*{Question 13}
\subsection*{Part a}
\begin{eqnarray*}
  & & \frac{r + \cos\theta + i\sin\theta}{1 + r\cos\theta - r\sin\theta} \\
  &=& \frac{r + \frac{z}{r}}{1 + \overline{z}} \\
  &=& \frac{r^2 + z}{r(1 + \overline{z})} \\  
  &=& \frac{z\overline{z} + z}{r(1 + \overline{z})} \\  
  &=& \frac{z(\overline{z} + 1)}{r(1 + \overline{z})} \\  
  &=& \frac{z}{r} \\  
  &=& \cos\theta + i\sin\theta
\end{eqnarray*}
\subsection*{Part b}
\begin{eqnarray*}
  & & \left(\frac{r + \sin\theta + i\cos\theta}{1 + r\sin\theta - r\cos\theta}\right)^n \\
  &=& \left(\frac{r + \cos\left(\frac{\pi}{2} - \theta\right) + i\sin\left(\frac{\pi}{2} - \theta\right)}{1 + r\cos\left(\frac{\pi}{2} - \theta\right) - r\sin\left(\frac{\pi}{2} - \theta\right)}\right)^n \\
  &=& \left(\cos\left(\frac{\pi}{2} - \theta\right) + i\sin\left(\frac{\pi}{2} - \theta\right)\right)^n \\
  &=& \cos\left(\frac{n\pi}{2} - n\theta\right) + i \sin\left(\frac{n\pi}{2} - n\theta\right)
\end{eqnarray*}
\subsection*{Part c}
\begin{eqnarray*}
  \left(\frac{r + \sin\theta + i\cos\theta}{1 + r\sin\theta - r\cos\theta}\right)^3 &=& \frac{\sqrt{3} + i}{2} \\
  \cos\left(\frac{3\pi}{2} - 3\theta\right) + i \sin\left(\frac{3\pi}{2} - 3\theta\right) &=& \frac{\sqrt{3} + i}{2} \\
  \frac{3\pi}{2} - 3\theta &=& \frac{\pi}{6} - 2k\pi \\
  3\theta &=& \frac{3\pi}{2} - \frac{\pi}{6} + 2k\pi \\
  3\theta &=& \frac{4\pi + 6k\pi}{3} \\
    \theta &=& \frac{4\pi + 6k\pi}{9}
\end{eqnarray*}
The result is independent of $ r $, so therefore $ r > 0 $. The graph is a line (excluding the origin) 
\subsection*{Part d}
It is impossible because the left hand side has modulus 1 but the right hand side has modulus 2.