\section*{Question 3}
\subsection*{Part a}
\begin{eqnarray*}
  \overrightarrow{m} \cdot \overrightarrow{n} &=& |\overrightarrow{m}| |\overrightarrow{n}| \cos(\frac{2 \pi}{3}) \\
                                              &=& 2 \times 1 \times \frac{-1}{2} \\
                                              &=& -1
\end{eqnarray*}
\subsection*{Part b}
\begin{eqnarray*}
  |\overrightarrow{p}| &=& \sqrt{\overrightarrow{p} \cdot \overrightarrow{p}} \\
                       &=& \sqrt{(3\overrightarrow{m} + 4\overrightarrow{n}) \cdot (3\overrightarrow{m} + 4\overrightarrow{n})} \\
                       &=& \sqrt{(9\overrightarrow{m} \cdot \overrightarrow{m} + 24\overrightarrow{m} \cdot\overrightarrow{n} + 16\overrightarrow{n} \cdot \overrightarrow{n})} \\
                       &=& \sqrt{(9|\overrightarrow{m}|^2 + 24\overrightarrow{m} \cdot\overrightarrow{n} + 16|\overrightarrow{n}|^2)} \\
                       &=& \sqrt{(9(2)^2 + 24(-1) + 16(1)^2)} \\
                       &=& \sqrt{(9(2)^2 + 24(-1) + 16(1)^2)} \\
                       &=& \sqrt{28}
\end{eqnarray*}
\begin{eqnarray*}
  |\overrightarrow{q}| &=& \sqrt{\overrightarrow{q} \cdot \overrightarrow{q}} \\
                       &=& \sqrt{(2\overrightarrow{m} - \overrightarrow{n}) \cdot (2\overrightarrow{m} - \overrightarrow{n})} \\
                       &=& \sqrt{(4\overrightarrow{m} \cdot \overrightarrow{m}  - 4\overrightarrow{m} \cdot\overrightarrow{n} + \overrightarrow{n} \cdot \overrightarrow{n})} \\
                       &=& \sqrt{(4|\overrightarrow{m}|^2 - 4\overrightarrow{m} \cdot\overrightarrow{n} + |\overrightarrow{n}|^2)} \\
                       &=& \sqrt{(4(2)^2 - 4(-1) + (1)^2)} \\
                       &=& \sqrt{21}
\end{eqnarray*}
\subsection*{Part c}
\begin{eqnarray*}
  \overrightarrow{p} \cdot \overrightarrow{q} &=& (3\overrightarrow{m} + 4\overrightarrow{n}) \cdot (2\overrightarrow{m} - \overrightarrow{n}) \\
  &=& 6\overrightarrow{m} \cdot \overrightarrow{m} - 3\overrightarrow{m} \cdot \overrightarrow{n} + 8\overrightarrow{n} \cdot \overrightarrow{m} - 4\overrightarrow{n} \cdot \overrightarrow{n} \\
  &=& 6|\overrightarrow{m}|^2 - 3\overrightarrow{m} \cdot \overrightarrow{n} + 8\overrightarrow{n} \cdot \overrightarrow{m} - 4|\overrightarrow{n}|^2 \\
  &=& 6(2)^2 - 3(-1) + 8(-1) - 4(1)^2 \\
  &=& 15
\end{eqnarray*}
Therefore, the area is :
\begin{eqnarray*}
  & & |\overrightarrow{p}| |\overrightarrow{q}| \sin(\theta) \\
  &=& \sqrt{|\overrightarrow{p}|^2 |\overrightarrow{q}|^2 \sin^2(\theta)} \\
  &=& \sqrt{|\overrightarrow{p}|^2 |\overrightarrow{q}|^2 (1-\cos^2(\theta))} \\
  &=& \sqrt{|\overrightarrow{p}|^2 |\overrightarrow{q}|^2 - |\overrightarrow{p}|^2 |\overrightarrow{q}|^2\cos^2(\theta)} \\
  &=& \sqrt{|\overrightarrow{p}|^2 |\overrightarrow{q}|^2 - (\overrightarrow{p} \cdot \overrightarrow{q})^2} \\
  &=& \sqrt{(28) (21) - (15)^2} \\
  &=& \sqrt{363} \\
  &=& 11 \sqrt{3}
\end{eqnarray*}