\documentclass{article}
\usepackage[utf8]{inputenc}
\usepackage{amsmath}

\title{Recurrence}
\author{Cecilia}
\date{June 2021}

\begin{document}
\maketitle

\section*{Problem}
Solve the recurrence $ a_k + \alpha a_{k-1} = (\alpha+1)^{k-3} (\alpha + 2) $ with $ a_0 = 1 $.

\section*{Solution}
\begin{eqnarray*}
                 f(x) &=& \sum\limits_{i=0}^{\infty} a_i x^i \\
                      &=& \sum\limits_{i=1}^{\infty} a_{i-1} x^{i-1} \\
        \alpha x f(x) &=& \sum\limits_{i=1}^{\infty} \alpha a_{i-1} x^i \\
                 f(x) &=& 1 + \sum\limits_{i=1}^{\infty} a_i x^i \\
  (\alpha x + 1) f(x) &=& 1 + \sum\limits_{i=1}^{\infty} (a_i + \alpha a_{i-1}) x^i \\
                      &=& 1 + \sum\limits_{i=1}^{\infty} (\alpha+1)^{i-3}(\alpha+2) x^i \\
                      &=& 1 + \frac{(\alpha+2)}{(\alpha+1)^3} \sum\limits_{i=1}^{\infty} ((\alpha+1)x)^i \\
                      &=& 1 + \frac{(\alpha+2)}{(\alpha+1)^3}\frac{(\alpha+1)x}{(1 - (\alpha+1)x)} \\
                      &=& 1 + \frac{(\alpha+2)x}{(\alpha+1)^2(1 - (\alpha+1)x)} \\
                 f(x) &=& \frac{1}{\alpha x + 1} + \frac{\alpha+2}{(\alpha+1)^2}\frac{x}{(1 - (\alpha+1)x)(\alpha x + 1)} \\
                      &=& \frac{1}{\alpha x + 1} + \frac{\alpha+2}{(\alpha+1)^2(2\alpha+1)}\left(\frac{1}{1 - (\alpha+1)x} - \frac{1}{\alpha x + 1}\right) \\
                      &=& \frac{1}{1 - (-\alpha x)} + \frac{\alpha+2}{(\alpha+1)^2(2\alpha+1)}\left(\frac{1}{1 - (\alpha+1)x} - \frac{1}{1 - (-\alpha x)}\right) \\
                      &=& \sum\limits_{i=0}^{\infty}(-\alpha x)^i + \frac{\alpha+2}{(\alpha+1)^2(2\alpha+1)}\left(\sum\limits_{i=0}^{\infty}((\alpha + 1)x)^i - \sum\limits_{i=0}^{\infty}(-\alpha x)^i\right) \\
                  a_i &=& (-\alpha)^i + \frac{\alpha+2}{(\alpha+1)^2(2\alpha+1)}\left((\alpha + 1)^i - (-\alpha)^i\right)
\end{eqnarray*}
\end{document}
