\section*{Question 3}
\begin{eqnarray*}
  & & \frac{||u + v||^2 - ||u - v||^2}{4} \\
  &=& \frac{\langle u + v, u + v \rangle - \langle u - v, u - v \rangle}{4} \\
  &=& \frac{\langle u, u \rangle + \langle u, v \rangle + \langle v,u \rangle + \langle v, v \rangle - \langle u, u \rangle + \langle u, v \rangle + \langle v, u \rangle - \langle v, v \rangle}{4} \\
  &=& \frac{\langle u, v \rangle + \langle v, u \rangle + \langle u, v \rangle + \langle v, u \rangle}{4} \\
  &=& \frac{\langle u, v \rangle + \langle u, v \rangle + \langle u, v \rangle + \langle u, v \rangle}{4} \\
  &=& \langle u, v \rangle
\end{eqnarray*}